pancake/panLangScript.sml
@@ -300,3 +300,8 @@ Definition free_var_ids_def:
   (free_var_ids (DecCall vn _ _ args p) = vn::free_var_ids p ++ FLAT (MAP var_exp args)) ∧
   (free_var_ids _ = [])
 End
+
+Definition inlinable_def:
+  inlinable (Function fi) = fi.inline ∧
+  inlinable (Decl _ _ _) = F
+End
