pancake/proofs/pan_to_crepProofScript.sml
@@ -3,6 +3,7 @@
 *)
 Theory pan_to_crepProof
 Ancestors
+  crep_inlineProof[qualified]
   panSem panProps crepLang crepSem pan_common
   listRange crepProps pan_commonProps pan_to_crep
 Libs
@@ -4471,18 +4472,29 @@ Theorem first_compile_prog_all_distinct:
   ALL_DISTINCT (MAP FST (functions prog)) ==>
   ALL_DISTINCT (MAP FST (pan_to_crep$compile_prog prog))
 Proof
-  fs [pan_to_crepTheory.compile_prog_def,MAP_MAP_o,ELIM_UNCURRY,o_DEF,ETA_AX]
+  fs [pan_to_crepTheory.compile_prog_def,MAP_MAP_o,ELIM_UNCURRY,o_DEF,ETA_AX,
+      pan_to_crepTheory.compile_to_crep_def,
+      crep_inlineTheory.compile_inl_prog_def]
+QED
+
+Theorem first_compile_to_crep_all_distinct:
+  ALL_DISTINCT (MAP FST (functions prog)) ==>
+  ALL_DISTINCT (MAP FST (pan_to_crep$compile_to_crep prog))
+Proof
+  fs [pan_to_crepTheory.compile_prog_def,MAP_MAP_o,ELIM_UNCURRY,o_DEF,ETA_AX,
+      pan_to_crepTheory.compile_to_crep_def,
+      crep_inlineTheory.compile_inl_prog_def]
 QED
 
 Theorem alookup_compile_prog_code:
   ALL_DISTINCT (MAP FST (functions pan_code)) ∧
   ALOOKUP (functions pan_code) start = SOME ([],prog) ==>
-  ALOOKUP (compile_prog pan_code) start =
+  ALOOKUP (compile_to_crep pan_code) start =
   SOME ([],
         comp_func (make_funcs(functions pan_code))
                   (get_eids(functions pan_code)) [] prog)
 Proof
-  rw[compile_prog_def, ctxt_fc_def,ELIM_UNCURRY,
+  rw[compile_to_crep_def, ctxt_fc_def,ELIM_UNCURRY,
      SIMP_RULE std_ss [ELIM_UNCURRY] ALOOKUP_MAP, crep_vars_def,
      panLangTheory.size_of_shape_def]
 QED
@@ -4490,7 +4502,7 @@ QED
 
 Theorem el_compile_prog_el_prog_eq:
   !prog n start cprog p.
-   EL n (compile_prog prog) = (start,[],cprog) /\
+   EL n (compile_to_crep prog) = (start,[],cprog) /\
    ALL_DISTINCT (MAP FST (functions prog)) /\ n < LENGTH(functions prog) /\
    ALOOKUP (functions prog) start = SOME ([],p) ==>
      EL n (functions prog) = (start,[],p)
@@ -4498,7 +4510,7 @@ Proof
   rw[] >>
   drule ALOOKUP_MEM >>
   strip_tac >>
-  gvs[compile_prog_def,EL_MAP,UNCURRY_eq_pair,
+  gvs[compile_to_crep_def,EL_MAP,UNCURRY_eq_pair,
       MEM_EL,EL_ALL_DISTINCT_EL_EQ,EL_MAP,SF DNF_ss] >>
   metis_tac[FST,SND,PAIR]
 QED
@@ -4509,13 +4521,13 @@ Theorem mk_ctxt_code_imp_code_rel:
   ⇒
   code_rel (mk_ctxt FEMPTY (make_funcs (functions pan_code)) 0 (get_eids (functions pan_code)))
            (alist_to_fmap (functions pan_code))
-           (alist_to_fmap (pan_to_crep$compile_prog pan_code))
+           (alist_to_fmap (pan_to_crep$compile_to_crep pan_code))
 Proof
   rw [code_rel_def, mk_ctxt_def] >>
   imp_res_tac ALOOKUP_MEM >>
   gvs[make_funcs_def,MAP2_MAP,ZIP_MAP_MAP,MAP_MAP_o,o_DEF,
       SIMP_RULE std_ss [ELIM_UNCURRY] ALOOKUP_MAP,ELIM_UNCURRY,
-      compile_prog_def,crep_vars_def,EVERY_MEM,comp_func_def,
+      compile_to_crep_def,crep_vars_def,EVERY_MEM,comp_func_def,
       mk_ctxt_def,ctxt_fc_def,make_vmap_def,list_max_i_genlist,EVERY_MEM] >>
   res_tac >> fs[]
 QED
@@ -4573,15 +4585,17 @@ Theorem compile_prog_distinct_params:
     EVERY (λ(name,params,body). ALL_DISTINCT params) (compile_prog prog)
 Proof
   rw[EVERY_MEM] >>
-  gvs[compile_prog_def,MEM_MAP,UNCURRY_eq_pair,crep_vars_def,ALL_DISTINCT_GENLIST]
+  gvs[compile_prog_def,MEM_MAP,UNCURRY_eq_pair,crep_vars_def,ALL_DISTINCT_GENLIST,
+      crep_inlineTheory.compile_inl_prog_def,
+      pan_to_crepTheory.compile_to_crep_def]
 QED
 
-Theorem state_rel_imp_semantics:
+Theorem state_rel_imp_semantics_to_crep:
   !(s:('a,'b) panSem$state) (t:('a,'b) crepSem$state) pan_code start.
     state_rel s t ∧
     ALL_DISTINCT (MAP FST (functions pan_code)) ∧
     s.code = alist_to_fmap(functions pan_code) ∧
-    t.code = alist_to_fmap (pan_to_crep$compile_prog pan_code) ∧
+    t.code = alist_to_fmap (pan_to_crep$compile_to_crep pan_code) ∧
     s.locals = FEMPTY ∧
     EVERY (localised_prog ∘ SND ∘ SND) (functions pan_code) ∧
     panLang$size_of_eids pan_code < dimword (:'a) /\
@@ -4843,6 +4857,71 @@ Proof
   cases_on ‘q’ >> fs [] >>
   cases_on ‘x’ >> fs [] >> rveq >> fs [] >>
    fs [state_rel_def, IS_PREFIX_THM]
+QED
+
+Theorem state_rel_imp_semantics_decls_to_crep:
+  !(s:('a,'b) panSem$state) (t:('a,'b) crepSem$state) pan_code start.
+    state_rel s t ∧
+    ALL_DISTINCT (MAP FST (functions pan_code)) ∧
+    s.code = FEMPTY ∧
+    t.code = alist_to_fmap (pan_to_crep$compile_to_crep pan_code) ∧
+    s.locals = FEMPTY ∧
+    EVERY (localised_prog ∘ SND ∘ SND) (functions pan_code) ∧
+    EVERY is_function pan_code ∧
+    panLang$size_of_eids pan_code < dimword (:'a) /\
+    FDOM s.eshapes =  FDOM (get_eids(functions pan_code)) ∧
+    semantics_decls s start pan_code <> Fail ==>
+      semantics t start = semantics_decls s start pan_code
+Proof
+  rw [semantics_decls_def] >>
+  gvs[AllCaseEqs(), GSYM IS_SOME_EQ_NOT_NONE, IS_SOME_EXISTS] >>
+  drule_all_then (gvs o single) evaluate_decls_only_functions >>
+  irule EQ_SYM >>
+  irule state_rel_imp_semantics_to_crep >>
+  simp[PULL_EXISTS] >>
+  first_assum $ irule_at $ Pos hd >>
+  simp[] >>
+  conj_tac
+  >- (rw[fmap_eq_flookup,FLOOKUP_FUPDATE_LIST,alookup_distinct_reverse] >>
+      TOP_CASE_TAC >> simp[]) >>
+  gvs[state_rel_def]
+QED
+
+Theorem state_rel_imp_semantics:
+  !(s:('a,'b) panSem$state) (t:('a,'b) crepSem$state) pan_code start.
+    state_rel s t ∧
+    ALL_DISTINCT (MAP FST (functions pan_code)) ∧
+    s.code = alist_to_fmap(functions pan_code) ∧
+    t.code = alist_to_fmap (pan_to_crep$compile_prog pan_code) ∧
+    s.locals = FEMPTY ∧
+    EVERY (localised_prog ∘ SND ∘ SND) (functions pan_code) ∧
+    panLang$size_of_eids pan_code < dimword (:'a) /\
+    FDOM s.eshapes =  FDOM (get_eids(functions pan_code)) ∧
+    semantics s start <> Fail ==>
+      semantics t start = semantics s start
+Proof
+  rw[pan_to_crepTheory.compile_prog_def] >>
+  qabbrev_tac `inl_funcs = MAP FST (functions (FILTER inlinable pan_code))` >>
+  qabbrev_tac `crep_code = compile_to_crep pan_code` >>
+  qabbrev_tac `inl_fs = alist_to_fmap (FILTER (λ(x, y). MEM x inl_funcs) crep_code)` >>
+  drule_at (Pos $ el 3) state_rel_imp_semantics_to_crep >>
+  disch_then $ drule_at (Pos last) >> fs[] >>
+  disch_then $ qspec_then `t with code := alist_to_fmap crep_code` mp_tac >> impl_tac
+  >- fs[state_rel_def] >>
+  disch_tac >>
+  qabbrev_tac `t_uninline = t with code := alist_to_fmap crep_code` >>
+  `semantics t_uninline start ≠ Fail` by fs[] >>
+  drule_at (Pos last) crep_inlineProofTheory.state_rel_imp_semantics >>
+  Cases_on `FLOOKUP t_uninline.code start` >> fs[]
+  >- fs[semantics_def, evaluate_def, lookup_code_def] >>
+  PairCases_on `x` >> fs[] >>
+  disch_then $ qspecl_then [`t`, `crep_code`, `inl_fs`] mp_tac >> impl_tac
+  >- (
+    fs[crep_inlineProofTheory.state_rel_code_def, state_rel_def,
+       crep_inlineProofTheory.locals_strong_rel_def, Abbr `t_uninline`] >>
+    imp_res_tac first_compile_to_crep_all_distinct >> fs[Abbr `crep_code`, Abbr `inl_fs`, SUBMAP_FLOOKUP_EQN, ALOOKUP_FILTER]
+  ) >>
+  rpt strip_tac >> fs[]
 QED
 
 Theorem state_rel_imp_semantics_decls:
